Source/Concurrency/YieldingProcDuplicator.cs
@@ -1,3 +1,4 @@
+using System;
 using System.Collections.Generic;
 using System.Linq;
 using System.Diagnostics;
@@ -123,36 +124,33 @@ namespace Microsoft.Boogie
     private Implementation enclosingImpl;
     private YieldingProc enclosingYieldingProc;
     private bool IsRefinementLayer => layerNum == enclosingYieldingProc.upperLayer;
-    private bool SummaryHasPendingAsyncParam => ((ActionProc) enclosingYieldingProc).refinedAction.HasPendingAsyncs;
+    private AtomicAction RefinedAction => ((ActionProc)enclosingYieldingProc).refinedAction;
+    private bool SummaryHasPendingAsyncParam => RefinedAction.HasPendingAsyncs;
     private List<Cmd> newCmdSeq;
 
-    private Variable returnedPAs;
+    private Dictionary<CtorType, Variable> returnedPAs;
 
-    private Variable ReturnedPAs
+    private Variable ReturnedPAs(CtorType pendingAsyncType)
     {
-      get
+      if (!returnedPAs.ContainsKey(pendingAsyncType))
       {
-        if (returnedPAs == null)
-        {
-          returnedPAs = civlTypeChecker.LocalVariable("returnedPAs", civlTypeChecker.pendingAsyncMultisetType);
-        }
-
-        return returnedPAs;
+        returnedPAs[pendingAsyncType] = civlTypeChecker.LocalVariable($"returnedPAs_{pendingAsyncType.Decl.Name}",
+          new MapType(Token.NoToken, new List<TypeVariable>(), new List<Type>() { pendingAsyncType }, Type.Int));
       }
+      return returnedPAs[pendingAsyncType];
     }
 
-    private Variable CollectedPAs
+    private Variable CollectedPAs(CtorType pendingAsyncType)
     {
-      get
+      if (!civlTypeChecker.implToPendingAsyncCollector[enclosingImpl].TryGetValue(pendingAsyncType, out var collectedPAs))
       {
-        if (!civlTypeChecker.implToPendingAsyncCollector.TryGetValue(enclosingImpl, out var collectedPAs))
-        {
-          collectedPAs = civlTypeChecker.LocalVariable("collectedPAs", civlTypeChecker.pendingAsyncMultisetType);
-          civlTypeChecker.implToPendingAsyncCollector[enclosingImpl] = collectedPAs;
-        }
-
-        return collectedPAs;
+        var pendingAsyncMultisetType = new MapType(Token.NoToken, new List<TypeVariable>(),
+          new List<Type>() { pendingAsyncType }, Type.Int);
+        collectedPAs =
+          civlTypeChecker.LocalVariable($"{pendingAsyncType.Decl.Name}_collectedPAs", pendingAsyncMultisetType);
+        civlTypeChecker.implToPendingAsyncCollector[enclosingImpl][pendingAsyncType] = collectedPAs;
       }
+      return collectedPAs;
     }
 
     public override Implementation VisitImplementation(Implementation impl)
@@ -162,7 +160,7 @@ namespace Microsoft.Boogie
       enclosingYieldingProc = civlTypeChecker.procToYieldingProc[impl.Proc];
       Debug.Assert(layerNum <= enclosingYieldingProc.upperLayer);
 
-      returnedPAs = null;
+      returnedPAs = new Dictionary<CtorType, Variable>();
 
       refinementCallCmds = new Dictionary<CallCmd, CallCmd>();
       Implementation newImpl = base.VisitImplementation(impl);
@@ -184,27 +182,14 @@ namespace Microsoft.Boogie
       }
 
       refinementCallCmds = null;
-
-      if (returnedPAs != null)
-      {
-        newImpl.LocVars.Add(returnedPAs);
-      }
+      
+      newImpl.LocVars.AddRange(returnedPAs.Values);
 
       if (enclosingYieldingProc is ActionProc && SummaryHasPendingAsyncParam && IsRefinementLayer)
       {
-        // TODO: This was copied from InductiveSequentialization property NoPendingAsyncs.
-        // Unify pending async stuff in something like PendingAsyncInstrumentation?
-        var paBound = civlTypeChecker.BoundVariable("pa", civlTypeChecker.pendingAsyncType);
-        var pa = Expr.Ident(paBound);
-        var expr = Expr.Eq(Expr.Select(Expr.Ident(CollectedPAs), pa), Expr.Literal(0));
-        var forallExpr = ExprHelper.ForallExpr(new List<Variable> {paBound}, expr);
-        forallExpr.Typecheck(new TypecheckingContext(null, Options));
-        newImpl.Blocks.First().Cmds.Insert(0, CmdHelper.AssumeCmd(forallExpr));
-
-        if (!impl.LocVars.Contains(CollectedPAs))
-        {
-          newImpl.LocVars.Add(CollectedPAs);
-        }
+        var assumeExpr = EmptyPendingAsyncMultisetExpr(CollectedPAs, RefinedAction.pendingAsyncs);
+        newImpl.LocVars.AddRange(civlTypeChecker.implToPendingAsyncCollector[impl].Values.Except(impl.LocVars));
+        newImpl.Blocks.First().Cmds.Insert(0, CmdHelper.AssumeCmd(assumeExpr));
       }
 
       absyMap[newImpl] = impl;
@@ -482,8 +467,8 @@ namespace Microsoft.Boogie
 
       if (refinedAction.HasPendingAsyncs)
       {
-        Debug.Assert(newCall.Outs.Count == newCall.Proc.OutParams.Count - 1);
-        CollectReturnedPendingAsyncs(newCall);
+        Debug.Assert(newCall.Outs.Count == newCall.Proc.OutParams.Count - refinedAction.pendingAsyncs.Count);
+        CollectReturnedPendingAsyncs(newCall, refinedAction);
       }
     }
 
@@ -523,10 +508,10 @@ namespace Microsoft.Boogie
       newCmdSeq.Add(new CommentCmd("injected gate >>>"));
     }
 
-    private void CollectReturnedPendingAsyncs(CallCmd newCall)
+    private void CollectReturnedPendingAsyncs(CallCmd newCall, AtomicAction refinedAction)
     {
       // Inject pending async collection
-      newCall.Outs.Add(Expr.Ident(ReturnedPAs));
+      newCall.Outs.AddRange(refinedAction.pendingAsyncs.Select(action => Expr.Ident(ReturnedPAs(action.pendingAsyncType))));
       if (!IsRefinementLayer)
       {
         return;
@@ -534,22 +519,34 @@ namespace Microsoft.Boogie
 
       if (SummaryHasPendingAsyncParam)
       {
-        var collectedUnionReturned = ExprHelper.FunctionCall(civlTypeChecker.pendingAsyncAdd,
-          Expr.Ident(CollectedPAs), Expr.Ident(ReturnedPAs));
-        newCmdSeq.Add(CmdHelper.AssignCmd(CollectedPAs, collectedUnionReturned));
+        var lhss = refinedAction.pendingAsyncs
+          .Select(action => new SimpleAssignLhs(Token.NoToken, Expr.Ident(CollectedPAs(action.pendingAsyncType))))
+          .ToList<AssignLhs>();
+        var rhss = refinedAction.pendingAsyncs.Select(action => ExprHelper.FunctionCall(action.pendingAsyncAdd,
+          Expr.Ident(CollectedPAs(action.pendingAsyncType)), Expr.Ident(ReturnedPAs(action.pendingAsyncType)))).ToList<Expr>();
+        newCmdSeq.Add(new AssignCmd(Token.NoToken, lhss, rhss));
       }
       else
       {
-        // TODO: As above, this was copied from InductiveSequentialization property NoPendingAsyncs.
-        // Unify pending async stuff in something like PendingAsyncInstrumentation?
-        var paBound = civlTypeChecker.BoundVariable("pa", civlTypeChecker.pendingAsyncType);
-        var pa = Expr.Ident(paBound);
-        var expr = Expr.Eq(Expr.Select(Expr.Ident(ReturnedPAs), pa), Expr.Literal(0));
-        var forallExpr = ExprHelper.ForallExpr(new List<Variable> {paBound}, expr);
-        forallExpr.Typecheck(new TypecheckingContext(null, civlTypeChecker.Options));
-        newCmdSeq.Add(CmdHelper.AssertCmd(newCall.tok, forallExpr,
+        newCmdSeq.Add(CmdHelper.AssertCmd(newCall.tok,
+          EmptyPendingAsyncMultisetExpr(ReturnedPAs, refinedAction.pendingAsyncs),
           "Pending asyncs created by this call are not summarized"));
       }
+    }
+
+    private Expr EmptyPendingAsyncMultisetExpr(Func<CtorType, Variable> pendingAsyncMultisets,
+      IEnumerable<AsyncAction> atomicActions)
+    {
+      var returnExpr = Expr.And(atomicActions.Select(action =>
+      {
+        var ctorType = action.pendingAsyncType;
+        var paBound = civlTypeChecker.BoundVariable("pa", ctorType);
+        var expr = Expr.Eq(Expr.Select(Expr.Ident(pendingAsyncMultisets(ctorType)), Expr.Ident(paBound)),
+          Expr.Literal(0));
+        return ExprHelper.ForallExpr(new List<Variable> { paBound }, expr);
+      }).ToList());
+      returnExpr.Typecheck(new TypecheckingContext(null, civlTypeChecker.Options));
+      return returnExpr;
     }
 
     private void AddDuplicateCall(CallCmd newCall, bool makeParallel)
@@ -588,24 +585,25 @@ namespace Microsoft.Boogie
 
     private void AddPendingAsync(CallCmd newCall, ActionProc actionProc)
     {
-      AtomicAction paAction;
+      AtomicAction atomicAction;
       if (actionProc.upperLayer == enclosingYieldingProc.upperLayer)
       {
-        paAction = actionProc.refinedAction;
+        atomicAction = actionProc.refinedAction;
       }
       else
       {
-        paAction = actionProc.RefinedActionAtLayer(layerNum);
+        atomicAction = actionProc.RefinedActionAtLayer(layerNum);
       }
 
-      if (paAction == civlTypeChecker.SkipAtomicAction)
+      if (atomicAction == civlTypeChecker.SkipAtomicAction)
       {
         return;
       }
 
+      var asyncAction = (AsyncAction)atomicAction;
       if (SummaryHasPendingAsyncParam)
       {
-        Expr[] newIns = new Expr[paAction.proc.InParams.Count];
+        Expr[] newIns = new Expr[atomicAction.proc.InParams.Count];
         for (int i = 0, j = 0; i < actionProc.proc.InParams.Count; i++)
         {
           if (civlTypeChecker.FormalRemainsInAction(actionProc, actionProc.proc.InParams[i]))
@@ -615,9 +613,10 @@ namespace Microsoft.Boogie
           }
         }
 
-        var pa = ExprHelper.FunctionCall(paAction.pendingAsyncCtor, newIns);
-        var inc = Expr.Add(Expr.Select(Expr.Ident(CollectedPAs), pa), Expr.Literal(1));
-        var add = CmdHelper.AssignCmd(CollectedPAs, Expr.Store(Expr.Ident(CollectedPAs), pa, inc));
+        var collectedPAs = CollectedPAs(asyncAction.pendingAsyncType);
+        var pa = ExprHelper.FunctionCall(asyncAction.pendingAsyncCtor, newIns);
+        var inc = Expr.Add(Expr.Select(Expr.Ident(collectedPAs), pa), Expr.Literal(1));
+        var add = CmdHelper.AssignCmd(collectedPAs, Expr.Store(Expr.Ident(collectedPAs), pa, inc));
         newCmdSeq.Add(add);
       }
       else
