Test/civl/inductive-sequentialization/paxos/PaxosSeq.bpl
@@ -8,14 +8,9 @@ modifies joinedNodes, voteInfo, decision;
 }
 
 procedure {:atomic}{:layer 2}
+{:creates "A_StartRound"}
 {:IS "A_Paxos'","INV"}
-{:elim "A_StartRound"}
-{:elim "A_Propose"}
-{:elim "A_Conclude"}
-{:elim "A_Join"}
-{:elim "A_Vote"}
 A_Paxos({:linear_in "perm"} rs: [Round]bool)
-returns ({:pending_async "A_StartRound"} PAs:[PA]int)
 {
   var {:pool "NumRounds"} numRounds: int;
   assert
@@ -24,46 +19,12 @@ returns ({:pending_async "A_StartRound"} PAs:[PA]int)
     {:add_to_pool "Round", 0, numRounds}
     {:add_to_pool "NumRounds", numRounds}
     0 <= numRounds;
-  PAs := (lambda pa: PA :: if pa is A_StartRound && pa->r == pa->r_lin && Round(pa->r) && pa->r <= numRounds then 1 else 0);
+  call create_asyncs((lambda pa: A_StartRound :: pa->r == pa->r_lin && Round(pa->r) && pa->r <= numRounds));
 }
 
-function {:inline} StartRoundPAs(k: int, numRounds: int) : [PA]int
-{
-  (lambda pa: PA :: if (pa is A_StartRound && pa->r == pa->r_lin && k < pa->r && pa->r <= numRounds) then 1 else 0)
-}
-
-function {:inline} StartRoundPlusJoinPlusProposePAs(k: int, m: Node, numRounds: int) : [PA]int
-{
-  (lambda pa : PA ::
-    if (pa is A_StartRound && pa->r == pa->r_lin && k+1 < pa->r && pa->r <= numRounds) ||
-       (pa == A_Propose(k+1, ProposePermissions(k+1))) ||
-       (pa is A_Join && pa->r == k+1 && m < pa->n && pa->n <= numNodes &&
-         pa->p == JoinPerm(k+1, pa->n))
-    then 1 else 0)
-}
-
-function {:inline} JoinOrProposeChoice(k: int, m: Node) : PA
-{
-  if m == numNodes then A_Propose(k+1, ProposePermissions(k+1)) else A_Join(k+1, m+1, JoinPerm(k+1, m+1))
-}
-
-function {:inline} StartRoundPlusVotePlusConcludePAs(k: int, m: Node, v: Value, numRounds: int) : [PA]int
-{
-  ( lambda pa: PA ::
-    if (pa is A_StartRound && pa->r == pa->r_lin && k+1 < pa->r && pa->r <= numRounds) ||
-       (pa == A_Conclude(k+1, v, ConcludePerm(k+1))) ||
-       (pa is A_Vote && pa->r == k+1 && m < pa->n && pa->n <= numNodes &&
-         pa->v == v && pa->p == VotePerm(k+1, pa->n))
-    then 1 else 0)
-}
-
-function {:inline} VoteOrConcludeChoice(k: int, m: Node, v: Value) : PA
-{
-  if m == numNodes then A_Conclude(k+1, v, ConcludePerm(k+1)) else A_Vote(k+1, m+1, v, VotePerm(k+1, m+1))
-}
-
-procedure {:IS_invariant}{:layer 2} INV({:linear_in "perm"} rs: [Round]bool)
-returns ({:pending_async "A_StartRound","A_Propose","A_Conclude","A_Join","A_Vote"} PAs:[PA]int, {:choice} choice:PA)
+procedure {:layer 2} {:creates "A_StartRound","A_Propose","A_Conclude","A_Join","A_Vote"}
+{:IS_invariant}{:elim "A_StartRound"}{:elim "A_Propose"}{:elim "A_Conclude"}{:elim "A_Join"}{:elim "A_Vote"}
+INV({:linear_in "perm"} rs: [Round]bool)
 modifies joinedNodes, voteInfo, decision;
 {
   var {:pool "NumRounds"} numRounds: int;
@@ -87,20 +48,23 @@ modifies joinedNodes, voteInfo, decision;
     0 <= k && k <= numRounds;
 
   if (k == numRounds) {
-      PAs := NoPAs();
+      // do nothing
   } else if (*) {
       assume
         (forall r: Round :: r < 1 || r > k ==> voteInfo[r] is None) &&
         (forall r: Round :: r < 1 || r > k ==> decision[r] is None);
-      PAs := StartRoundPAs(k, numRounds);
-      choice := A_StartRound(k+1, k+1);
+      call create_asyncs((lambda pa: A_StartRound :: pa->r == pa->r_lin && k < pa->r && pa->r <= numRounds));
+      call set_choice(A_StartRound(k+1, k+1));
   } else if (*) {
       assume
         (forall r: Round :: r < 1 || r > k ==> voteInfo[r] is None) &&
         (forall r: Round :: r < 1 || r > k ==> decision[r] is None);
       assume {:add_to_pool "Node", m} 0 <= m && m <= numNodes;
-      PAs := StartRoundPlusJoinPlusProposePAs(k, m, numRounds);
-      choice := JoinOrProposeChoice(k, m);
+      call create_asyncs((lambda pa: A_StartRound :: pa->r == pa->r_lin && k+1 < pa->r && pa->r <= numRounds));
+      call create_async(A_Propose(k+1, ProposePermissions(k+1)));
+      call create_asyncs((lambda pa: A_Join :: pa->r == k+1 && m < pa->n && pa->n <= numNodes && pa->p == JoinPerm(k+1, pa->n)));
+      if (m == numNodes) { call set_choice(A_Propose(k+1, ProposePermissions(k+1))); }
+      else { call set_choice(A_Join(k+1, m+1, JoinPerm(k+1, m+1))); }
   } else {
       assume
         voteInfo[k+1] is Some &&
@@ -109,8 +73,11 @@ modifies joinedNodes, voteInfo, decision;
       assume {:add_to_pool "Node", m}
         0 <= m && m <= numNodes &&
         (forall n: Node :: n < 1 || n > m ==> !voteInfo[k+1]->t->ns[n]);
-      PAs := StartRoundPlusVotePlusConcludePAs(k, m, voteInfo[k+1]->t->value, numRounds);
-      choice := VoteOrConcludeChoice(k, m, voteInfo[k+1]->t->value);
+      call create_asyncs((lambda pa: A_StartRound :: pa->r == pa->r_lin && k+1 < pa->r && pa->r <= numRounds));
+      call create_async(A_Conclude(k+1, voteInfo[k+1]->t->value, ConcludePerm(k+1)));
+      call create_asyncs((lambda pa: A_Vote :: pa->r == k+1 && m < pa->n && pa->n <= numNodes && pa->v == voteInfo[k+1]->t->value && pa->p == VotePerm(k+1, pa->n)));
+      if (m == numNodes) { call set_choice(A_Conclude(k+1, voteInfo[k+1]->t->value, ConcludePerm(k+1))); }
+      else { call set_choice(A_Vote(k+1, m+1, voteInfo[k+1]->t->value, VotePerm(k+1, m+1))); }
   }
 
   // If there was a decision for some value, then there must have been a
